src/tls/Test.StAE.fst
@@ -36,9 +36,9 @@ let nprint s : St unit = print s
 private let pre_id (role:role) =
   let cr  = Bytes.create 32ul 0z in
   let sr  = Bytes.create 32ul 0z in
-  let kdf = PRF_TLS_1p2 kdf_label (HMac Hashing.Spec.SHA256) in
+  let kdf = PRF_TLS_1p2 kdf_label Hashing.Spec.SHA256 in
   let msid = StandardMS PMS.DummyPMS (cr @| sr) kdf in
-  ID12 TLS_1p2 msid kdf (AEAD CoreCrypto.AES_256_GCM Hashing.Spec.SHA256) cr sr role
+  ID12 TLS_1p2 msid kdf (AEAD EverCrypt.AES256_GCM Hashing.Spec.SHA256) cr sr role
 
 let id12 = pre_id Client
 
@@ -47,7 +47,7 @@ let id13 =
   let ch0 = {
     li_ch0_cr = cr;
     li_ch0_ed_psk = Bytes.utf8_encode "whatever";
-    li_ch0_ed_ae = CoreCrypto.AES_256_GCM;
+    li_ch0_ed_ae = EverCrypt.AES256_GCM;
     li_ch0_ed_hash = Hashing.Spec.SHA256; } in
   let li = LogInfo_CH0 ch0 in
   let i = ExpandedSecret
